Complements.thy
@@ -1,0 +1,193 @@
+
+theory Complements
+  imports AutoCorres.AutoCorres
+begin
+
+lemma gets_comp : "do x <- gets f ;
+                     gets (f' x) od
+                     =
+                  gets (\<lambda> s . f' (f s) s)"
+  by monad_eq
+
+
+lemma gets_return : "do x <- gets f ;
+                     return (g x) od = gets (g o f)"
+  by monad_eq
+
+
+ML \<open>
+fun called_funs g fn_name =
+    case Symtab.lookup g fn_name of
+   SOME t => Binaryset.listItems t
+   | NONE => []
+
+fun rec_called_funs g fn_name =
+  let
+    val l =  called_funs g fn_name
+  in
+  l @ (List.map (rec_called_funs g) l
+  |> List.concat)
+end
+
+fun get_callgraph thy Cfile =
+ CalculateState.get_csenv thy Cfile
+  |> the |> ProgramAnalysis.compute_callgraphs |> #callgraph
+
+
+(*
+fun called_funs_theory thy Cfile fn_name =
+get_callgraph thy Cfile |> (fn g => rec_called_funs g fn_name)
+*)
+\<close>
+
+
+
+ML \<open>val suffix_def_easy = "'_def'"\<close>
+ML \<open>fun easy_def ctxt (name : string) : thm = 
+Proof_Context.get_thm ctxt (name ^ suffix_def_easy)
+\<close>
+
+ML \<open>fun normal_def ctxt (name : string) : thm = 
+Proof_Context.get_thm ctxt (name ^ "'_def")
+\<close>
+
+ML \<open>
+fun my_of ctxt vars = 
+  Rule_Insts.of_rule ctxt (List.map SOME vars, []) []
+
+fun my_simp ctxt thms = 
+Simplifier.asm_simplify ((* clear_simpset *) ctxt addsimps thms)
+
+fun my_THEN thm2 thm1 =
+thm1 RSN (1 , thm2) ;
+
+fun my_OF thm1 thms =
+thm1 OF thms ;
+\<close>
+
+lemma complicated : "\<And> P Q f. P f \<Longrightarrow> Q f \<Longrightarrow> Q f"
+  by simp
+
+ML \<open>
+(* 
+replace a goal A \<Rightarrow> B \<Rightarrow> P f with
+A \<Rightarrow> B \<Rightarrow> Q f \<Rightarrow> Q f, for sP the string defining P
+(typically a lambda, and sQ the string defining Q)
+*)
+fun unify_goal_and_prove ctxt sP sQ (* simps *) thm =
+  thm |> my_THEN
+(
+Proof_Context.get_thm ctxt "complicated"
+|> my_of ctxt [sP, "_", sQ]
+|> Simplifier.asm_full_simplify
+(ctxt (*addsimps simps *))
+) 
+
+(* 
+replace a goal A \<Rightarrow> B \<Rightarrow> P f with
+A \<Rightarrow> B \<Rightarrow> undefined = Q f \<Rightarrow> undefined = Q f,
+ for sP the string defining P
+(typically a lambda, and sQ the string defining Q)
+*)
+fun unify_goal_and_prove_eq ctxt sP sQ  =
+  unify_goal_and_prove ctxt sP 
+    ("\<lambda> f.  undefined = " ^ sQ ^ " f") 
+\<close>
+
+
+ML \<open>
+(* generate the isabelle getter term depending on w by inspecting the
+ C getter definition.
+lget_aa is the list of constants to be unfolded in the
+getter_name definition
+*)
+fun generate_getter_term ctxt getter_name lget_aa heap_getter =
+easy_def ctxt getter_name
+|> 
+Rule_Insts.of_rule ctxt ([SOME "ptr"], []) [] |>
+my_simp ctxt
+([
+(* We add this rewrite rule to remove the guards *)
+  (Proof_Context.read_term_pattern ctxt 
+   "\<And> (e :: lifted_globals \<Rightarrow> _). guard e = gets (\<lambda>_  . ())"
+  |> Thm.cterm_of ctxt  |> Thm.assume)
+  ] 
+  @ @{thms gets_return gets_comp } 
+ @ (List.map (easy_def ctxt) lget_aa))
+(* Here we should have a conclusion of the shape
+getter ptr = gets (\<lambda>s . f s)
+
+
+*)
+|> unify_goal_and_prove_eq ctxt 
+("(\<lambda> f. " ^ getter_name ^ "' ptr = gets (\<lambda>s . f  (" ^ heap_getter ^ " s ptr)))")
+"(\<lambda> f. f w)" 
+
+|> Thm.concl_of 
+|> Utils.rhs_of_eq
+\<close>
+
+
+
+
+
+lemma modify_comp: "do _ <- modify f ; modify f' od = modify (f' o f )"
+  by (monad_eq)
+
+lemma ptr_set_comp :
+   "(\<lambda>x. x(ptr := f (x ptr))) o (\<lambda>x. x(ptr := f' (x ptr))) = (\<lambda>x. x(ptr := f (f' (x ptr))))"
+(*  proof obtained by sledgehammer *)
+proof -
+have "\<forall>fa. ((\<lambda>fa. fa(ptr := f (fa ptr))) \<circ> (\<lambda>f. f(ptr := f' (f ptr)))) fa = fa(ptr := f (f' (fa ptr)))"
+  by (simp add: fun_upd_same)
+  then show ?thesis
+    by blast
+qed
+
+ML \<open>
+(* generate the isabelle getter term depending on w and (v the new value) by inspecting the
+ C getter definition.
+lget_aa is the list of constants to be unfolded in the
+getter_name definition
+*)
+(*fun generate_setter_term ctxt setter_name lset_aa  =*)
+fun generate_setter_term ctxt setter_name lset_aa heap_setter =
+normal_def ctxt setter_name
+|> 
+Rule_Insts.of_rule ctxt ([SOME "ptr", SOME "v"], []) [] |>
+my_simp ctxt
+([
+(* We add this rewrite rule to remove the guards *)
+  (Proof_Context.read_term_pattern ctxt 
+   "\<And> (e :: lifted_globals \<Rightarrow> _). guard e = gets (\<lambda>_  . ())"
+  |> Thm.cterm_of ctxt  |> Thm.assume)
+  ] 
+  @ @{thms modify_comp (* heap_t1_C_update_comp *) ptr_set_comp
+(* t1_C_updupd_same *)
+ } 
+ @ (List.map (normal_def ctxt) lset_aa))
+(* Here we should have a conclusion of the shape
+getter ptr = gets (\<lambda>s . f s)
+
+
+*)
+|> my_THEN @{thm  HOL.meta_eq_to_obj_eq}
+|> unify_goal_and_prove_eq ctxt 
+("(\<lambda> f. " ^ setter_name ^ 
+"' ptr v = modify (" ^ heap_setter ^ " (\<lambda>x . x(ptr := f  (x ptr)))))")
+"(\<lambda> f. f w)" 
+
+|> Thm.concl_of 
+|> Utils.rhs_of_eq
+\<close>
+
+
+ML \<open>
+fun my_generate_fun name vars term ctxt = 
+ case Utils.define_const_args name false term
+(List.map (fn x => (x , Term.dummyT)) vars) ctxt of
+   (_,_,ctxt) => ctxt 
+ \<close>
+
+
+end
